theories/diffpriv/examples/list.v
@@ -765,7 +765,7 @@ Section list_specs.
       simpl in Ha; subst; rewrite /list_nth; tp_pures; rewrite -/list_nth.
     - iApply spec_update_ret. iFrame. iLeft. iPureIntro. split; [done|simpl; lia].
     - destruct Ha as [lv' [Hlv Hlcoh]]; subst.
-      tp_pures; first naive_solver. case_bool_decide; tp_pures.
+      tp_pures. case_bool_decide; tp_pures.
       + iApply spec_update_ret. iFrame. iRight. iPureIntro. simplify_eq.
         replace i with 0%nat; last lia. simpl. naive_solver.
       + destruct i; first done.
@@ -882,7 +882,6 @@ Section list_specs.
     - destruct Hl as [lv' [Hlv Hlcoh]]; subst.
       rewrite /list_remove_nth.
       tp_pures.
-      { rewrite /vals_compare_safe /val_is_unboxed /lit_is_unboxed. auto. }
       fold list_remove_nth.
       case_bool_decide; tp_pures.
       + iModIntro.
